Cslib/Computability/LambdaCalculus/LocallyNameless/Stlc/Context.lean
@@ -47,11 +47,11 @@ theorem dom_perm_mem_iff (h : Γ.Perm Δ) {x : Var} :
 omit [DecidableEq Var] in
 /-- Context well-formedness is preserved on permuting a context. -/
 @[aesop safe forward (rule_sets := [LambdaCalculus.LocallyNameless.ruleSet])]
-theorem perm (h : Γ.Perm Δ) : Γ✓ → Δ✓ := (List.perm_nodupKeys h).mp
+theorem wf_perm (h : Γ.Perm Δ) : Γ✓ → Δ✓ := (List.perm_nodupKeys h).mp
 
 omit [DecidableEq Var] in
 @[aesop safe forward (rule_sets := [LambdaCalculus.LocallyNameless.ruleSet])]
-theorem strengthen : (Δ ++ ⟨x, σ⟩ :: Γ)✓ → (Δ ++ Γ)✓ := by
+theorem wf_strengthen : (Δ ++ ⟨x, σ⟩ :: Γ)✓ → (Δ ++ Γ)✓ := by
   intros ok
   have sl : List.Sublist (Δ ++ Γ) (Δ ++ ⟨x, σ⟩ :: Γ) := by simp
   exact List.NodupKeys.sublist sl ok
